theories/ftlr/Mov.v
@@ -12,13 +12,14 @@ Section fundamental.
     {Σ:gFunctors}
     {ceriseg:ceriseG Σ} {sealsg: sealStoreG Σ}
     {Cname : CmptNameG}
-    {stsg : STSG Addr region_type Σ} {heapg : heapGS Σ}
+    {stsg : STSG Addr region_type Σ} {tframeg : TFRAMEG Σ} {heapg : heapGS Σ}
     {nainv: logrel_na_invs Σ}
     `{MP: MachineParameters}.
 
   Notation STS := (leibnizO (STS_states * STS_rels)).
   Notation STS_STD := (leibnizO (STS_std_states Addr region_type)).
-  Notation WORLD := (prodO STS_STD STS).
+  Notation TFRAME := (leibnizO nat).
+  Notation WORLD := ( prodO (prodO STS_STD STS) TFRAME) .
   Implicit Types W : WORLD.
   Implicit Types C : CmptName.
 
@@ -33,7 +34,7 @@ Section fundamental.
     ftlr_instr W C regs p p' g b e a w (Mov dst src) ρ P.
   Proof.
     intros Hp Hsome HcorrectPC Hbae Hfp HO Hpers Hpwl Hregion Hnotrevoked Hi.
-    iIntros "#IH #Hinv_interp #Hreg #Hinva #Hrcond #Hwcond #Hmono #HmonoV Hw Hsts Hown".
+    iIntros "#IH #Hinv_interp #Hreg #Hinva #Hrcond #Hwcond #Hmono #HmonoV Hw Hsts Htframe Hown".
     iIntros "Hr Hstate Ha HPC Hmap".
     iInsert "Hmap" PC.
     iApply (wp_Mov with "[$Ha $Hmap]"); eauto.
@@ -61,7 +62,7 @@ Section fundamental.
         { destruct ρ;auto;contradiction. }
         destruct (decide (r = PC)).
         { simplify_map_eq.
-          iApply ("IH" $! _ _ regs with "[%] [] [Hmap] [$Hr] [$Hsts] [$Hown]"); eauto.
+          iApply ("IH" $! _ _ regs with "[%] [] [Hmap] [$Hr] [$Hsts] [$Htframe] [$Hown]"); eauto.
           iApply (interp_next_PC with "Hinv_interp"); eauto.
         }
         simplify_map_eq.
@@ -75,13 +76,13 @@ Section fundamental.
           iApply wp_value;auto.
         }
 
-        iApply ("IH" $! _ _ regs with "[%] [] [Hmap] [$Hr] [$Hsts] [$Hown]"); eauto.
+        iApply ("IH" $! _ _ regs with "[%] [] [Hmap] [$Hr] [$Hsts] [$Htframe] [$Hown]"); eauto.
         iApply (interp_weakening with "IH Hr0"); eauto; try reflexivity; try solve_addr.
       }
       { map_simpl "Hmap".
         iDestruct (region_close with "[$Hstate $Hr $Ha $HmonoV Hw]") as "Hr"; eauto.
         { destruct ρ;auto;contradiction. }
-        iApply ("IH" $! _ _ (<[dst:=w0]> _) with "[%] [] [Hmap] [$Hr] [$Hsts] [$Hown]"); eauto.
+        iApply ("IH" $! _ _ (<[dst:=w0]> _) with "[%] [] [Hmap] [$Hr] [$Hsts] [$Htframe] [$Hown]"); eauto.
         - intros; simpl.
           rewrite lookup_insert_is_Some.
           destruct (decide (dst = x)); auto; right; split; auto.
