theories/ftlr/ReadSR.v
@@ -12,13 +12,14 @@ Section fundamental.
     {Σ:gFunctors}
     {ceriseg:ceriseG Σ} {sealsg: sealStoreG Σ}
     {Cname : CmptNameG}
-    {stsg : STSG Addr region_type Σ} {heapg : heapGS Σ}
+    {stsg : STSG Addr region_type Σ} {tframeg : TFRAMEG Σ} {heapg : heapGS Σ}
     {nainv: logrel_na_invs Σ}
     `{MP: MachineParameters}.
 
   Notation STS := (leibnizO (STS_states * STS_rels)).
   Notation STS_STD := (leibnizO (STS_std_states Addr region_type)).
-  Notation WORLD := (prodO STS_STD STS).
+  Notation TFRAME := (leibnizO nat).
+  Notation WORLD := ( prodO (prodO STS_STD STS) TFRAME) .
   Implicit Types W : WORLD.
   Implicit Types C : CmptName.
 
@@ -33,11 +34,11 @@ Section fundamental.
     ftlr_instr W C regs p p' g b e a w (ReadSR dst src) ρ P.
   Proof.
     intros Hp Hsome HcorrectPC Hbae Hfp HO Hpers Hpwl Hregion Hnotrevoked Hi.
-    iIntros "#IH #Hinv_interp #Hreg #Hinva #Hrcond #Hwcond #Hmono #HmonoV Hw Hsts Hown".
+    iIntros "#IH #Hinv_interp #Hreg #Hinva #Hrcond #Hwcond #Hmono #HmonoV Hw Hsts Htframe Hown".
     iIntros "Hr Hstate Ha HPC Hmap".
     iInsert "Hmap" PC.
     destruct (has_sreg_access p) eqn:HpXRS.
-    { iClear "IH Hreg Hinva Hrcond Hwcond Hmono HmonoV Hw Hsts Hown Hr Hstate Ha Hmap".
+    { iClear "IH Hreg Hinva Hrcond Hwcond Hmono HmonoV Hw Hsts Htframe Hown Hr Hstate Ha Hmap".
       iEval (rewrite !fixpoint_interp1_eq interp1_eq) in "Hinv_interp".
       destruct (isO p) eqn: HnO.
       { destruct Hp as [Hexec _]
