theories/ftlr/Seal.v
@@ -11,13 +11,14 @@ Section fundamental.
     {Σ:gFunctors}
     {ceriseg:ceriseG Σ} {sealsg: sealStoreG Σ}
     {Cname : CmptNameG}
-    {stsg : STSG Addr region_type Σ} {heapg : heapGS Σ}
+    {stsg : STSG Addr region_type Σ} {tframeg : TFRAMEG Σ} {heapg : heapGS Σ}
     {nainv: logrel_na_invs Σ}
     `{MP: MachineParameters}.
 
   Notation STS := (leibnizO (STS_states * STS_rels)).
   Notation STS_STD := (leibnizO (STS_std_states Addr region_type)).
-  Notation WORLD := (prodO STS_STD STS).
+  Notation TFRAME := (leibnizO nat).
+  Notation WORLD := ( prodO (prodO STS_STD STS) TFRAME) .
   Implicit Types W : WORLD.
   Implicit Types C : CmptName.
 
@@ -55,7 +56,7 @@ Section fundamental.
     ftlr_instr W C regs p p' g b e a w (Seal dst r1 r2) ρ P.
   Proof.
     intros Hp Hsome HcorrectPC Hbae Hfp HO Hpers Hpwl Hregion Hnotrevoked Hi.
-    iIntros "#IH #Hinv_interp #Hreg #Hinva #Hrcond #Hwcond #Hmono #HmonoV Hw Hsts Hown".
+    iIntros "#IH #Hinv_interp #Hreg #Hinva #Hrcond #Hwcond #Hmono #HmonoV Hw Hsts Htframe Hown".
     iIntros "Hr Hstate Ha HPC Hmap".
     iInsert "Hmap" PC.
     iApply (wp_Seal with "[$Ha $Hmap]"); eauto.
@@ -92,7 +93,7 @@ Section fundamental.
       { destruct ρ;auto;contradiction. }
 
       iApply ("IH" $! _ _ (<[dst := _]> (<[PC := _]> regs))
-               with "[%] [] [Hmap] [$Hr] [$Hsts] [$Hown]")
+               with "[%] [] [Hmap] [$Hr] [$Hsts] [$Htframe] [$Hown]")
       ; eauto.
       + intro; cbn. by repeat (rewrite lookup_insert_is_Some'; right).
       + iIntros (ri wi Hri Hregs_ri).
