theories/ftlr/UnSeal.v
@@ -11,13 +11,14 @@ Section fundamental.
     {Σ:gFunctors}
     {ceriseg:ceriseG Σ} {sealsg: sealStoreG Σ}
     {Cname : CmptNameG}
-    {stsg : STSG Addr region_type Σ} {heapg : heapGS Σ}
+    {stsg : STSG Addr region_type Σ} {tframeg : TFRAMEG Σ} {heapg : heapGS Σ}
     {nainv: logrel_na_invs Σ}
     `{MP: MachineParameters}.
 
   Notation STS := (leibnizO (STS_states * STS_rels)).
   Notation STS_STD := (leibnizO (STS_std_states Addr region_type)).
-  Notation WORLD := (prodO STS_STD STS).
+  Notation TFRAME := (leibnizO nat).
+  Notation WORLD := ( prodO (prodO STS_STD STS) TFRAME) .
   Implicit Types W : WORLD.
   Implicit Types C : CmptName.
 
@@ -56,7 +57,7 @@ Section fundamental.
     ftlr_instr W C regs p p' g b e a w (UnSeal dst r1 r2) ρ P.
   Proof.
     intros Hp Hsome HcorrectPC Hbae Hfp HO Hpers Hpwl Hregion Hnotrevoked Hi.
-    iIntros "#IH #Hinv_interp #Hreg #Hinva #Hrcond #Hwcond #Hmono #HmonoV Hw Hsts Hown".
+    iIntros "#IH #Hinv_interp #Hreg #Hinva #Hrcond #Hwcond #Hmono #HmonoV Hw Hsts Htframe Hown".
     iIntros "Hr Hstate Ha HPC Hmap".
     iInsert "Hmap" PC.
     iApply (wp_UnSeal with "[$Ha $Hmap]"); eauto.
@@ -93,7 +94,7 @@ Section fundamental.
     { (* PC ≠ dst *)
       simplify_map_eq; map_simpl "Hmap".
       iApply ("IH" $! _ _ (<[dst:=WSealable sb]> regs)
-               with "[%] [] [Hmap] [$Hr] [$Hsts] [$Hown]")
+               with "[%] [] [Hmap] [$Hr] [$Hsts] [$Htframe] [$Hown]")
       ; eauto.
       + cbn; intros. by repeat (rewrite lookup_insert_is_Some'; right).
       + iIntros (ri v Hri Hvs).
@@ -111,7 +112,7 @@ Section fundamental.
     { (* PC = dst *)
       simplify_map_eq; map_simpl "Hmap".
       destruct (executeAllowed p'') eqn:Hpft.
-      - iApply ("IH" $! _ _ regs with "[%] [] [Hmap] [$Hr] [$Hsts] [$Hown]")
+      - iApply ("IH" $! _ _ regs with "[%] [] [Hmap] [$Hr] [$Hsts] [$Htframe] [$Hown]")
         ; eauto.
         iApply (interp_weakening with "IH HVsb"); eauto; try solve_addr; try done.
       - (* not executable *)
