theories/multiple_updates.v
@@ -1,5 +1,5 @@
 From iris.proofmode Require Import tactics.
-From cap_machine Require Import logrel.
+From cap_machine Require Import region_invariants.
 Require Import Eqdep_dec List.
 From stdpp Require Import countable.
 
@@ -11,13 +11,14 @@ Section std_updates.
   Context {Σ:gFunctors}
     {ceriseg:ceriseG Σ}
     {Cname : CmptNameG}
-    {stsg : STSG Addr region_type Σ}
+    {stsg : STSG Addr region_type Σ} {tframeg : TFRAMEG Σ}
     {heapg : heapGS Σ}
     `{MP: MachineParameters}.
 
   Notation STS := (leibnizO (STS_states * STS_rels)).
   Notation STS_STD := (leibnizO (STS_std_states Addr region_type)).
-  Notation WORLD := (prodO STS_STD STS).
+  Notation TFRAME := (leibnizO nat).
+  Notation WORLD := ( prodO (prodO STS_STD STS) TFRAME) .
   Implicit Types W : WORLD.
   Implicit Types C : CmptName.
 
@@ -30,32 +31,38 @@ Section std_updates.
    Definition std_update_temp_multiple W l := std_update_multiple W l Temporary.
 
    Lemma std_update_multiple_loc_sta W l ρ :
-     (std_update_multiple W l ρ).2.1 = W.2.1.
+     loc (std_update_multiple W l ρ) = loc W.
    Proof.
      induction l; auto.
    Qed.
 
    Lemma std_update_multiple_loc_rel W l ρ :
-     (std_update_multiple W l ρ).2.2 = W.2.2.
+     wrel (std_update_multiple W l ρ) = wrel W.
    Proof.
      induction l; auto.
    Qed.
 
-   Lemma std_update_multiple_loc W l ρ :
-     (std_update_multiple W l ρ).2 = W.2.
+   Lemma std_update_multiple_cus W l ρ :
+     cus (std_update_multiple W l ρ) = cus W.
    Proof.
      induction l; auto.
    Qed.
 
-   Lemma std_update_multiple_proj_eq W Wloc l ρ :
-     ((std_update_multiple W l ρ).1, Wloc) = std_update_multiple (W.1,Wloc) l ρ.
+   Lemma std_update_multiple_frm W l ρ :
+     frm (std_update_multiple W l ρ) = frm W.
    Proof.
-     destruct W as [Wsta Wloc']. simpl. induction l; auto.
+     induction l; auto.
+   Qed.
+
+   Lemma std_update_multiple_proj_eq W Wloc Wfrm l ρ :
+     ( ( std (std_update_multiple W l ρ) , Wloc), Wfrm) = std_update_multiple ( (std W, Wloc), Wfrm) l ρ.
+   Proof.
+     destruct W as [ [Wsta Wloc'] Wfrm']. simpl. induction l; auto.
      simpl. rewrite -IHl. auto.
    Qed.
 
-   Lemma std_update_multiple_std_sta_eq W Wloc l ρ :
-     (std_update_multiple W l ρ).1 = (std_update_multiple (W.1, Wloc) l ρ).1.
+   Lemma std_update_multiple_std_sta_eq W Wloc Wfrm l ρ :
+     std (std_update_multiple W l ρ) = std (std_update_multiple ((std W, Wloc), Wfrm) l ρ).
    Proof.
      destruct W as [Wsta Wloc']. simpl. induction l; auto.
      simpl. rewrite -IHl. auto.
@@ -229,7 +236,8 @@ Section std_updates.
        destruct (decide (a ∈ l)).
        { rewrite (_: <s[a:=ρ]s>(std_update_multiple W l ρ) = std_update_multiple W l ρ) /=.
          by apply related_sts_pub_refl_world.
-         rewrite /std_update insert_id /=. by destruct (std_update_multiple W l ρ).
+         rewrite /std_update insert_id /=.
+         by destruct (std_update_multiple W l ρ) as [ [] ].
          by apply std_sta_update_multiple_lookup_in_i. }
        apply related_sts_pub_world_fresh; auto.
        intros Hcontr. apply std_update_multiple_not_in_sta in Hcontr; auto.
@@ -243,7 +251,7 @@ Section std_updates.
      apply elem_of_list_lookup_2 in Helem.
      apply elem_of_list_split in Helem as [l1 [l2 Heq] ].
      rewrite Heq std_update_multiple_swap /= /std_update.
-     rewrite /std /=. rewrite lookup_insert. auto.
+     rewrite /=. rewrite lookup_insert. auto.
    Qed.
 
 
@@ -287,11 +295,16 @@ Section std_updates.
      related_sts_pub_world (std_update_multiple W l ρ) (std_update_multiple W' l ρ).
    Proof.
      intros Hrelated.
-     destruct W as [ Wstd_sta [Wloc_sta Wloc_rel] ].
-     destruct W' as [ Wstd_sta' [Wloc_sta' Wloc_rel'] ].
-     destruct Hrelated as [ [Hstd_dom1 Hstd_related ] Hloc_related].
+     destruct W as [ [Wstd_sta [Wloc_sta Wloc_rel] ] Wfrm ].
+     destruct W' as [ [ Wstd_sta' [Wloc_sta' Wloc_rel'] ] Wfrm' ].
+     destruct Hrelated as [ [ [Hstd_dom1 Hstd_related ] Hcus_related]  Hfrm_related ].
      simpl in *.
-     split;[clear Hloc_related|by repeat rewrite std_update_multiple_loc_rel std_update_multiple_loc_sta].
+     split; [split|];[clear Hcus_related|by repeat rewrite std_update_multiple_loc_rel std_update_multiple_loc_sta|].
+     2: { rewrite !/related_tframe_pub in Hfrm_related |- *
+          ; rewrite !std_update_multiple_frm
+          ; simplify_eq.
+          done.
+     }
      split.
      - apply std_update_multiple_std_sta_dom_monotone. auto.
      - intros i x y Hx Hy.
@@ -299,8 +312,8 @@ Section std_updates.
        + rewrite std_sta_update_multiple_lookup_in_i in Hx;auto.
          rewrite std_sta_update_multiple_lookup_in_i in Hy;auto.
          inversion Hx; inversion Hy; subst. left.
-       + rewrite std_sta_update_multiple_lookup_same_i /std /= in Hx;auto.
-         rewrite std_sta_update_multiple_lookup_same_i /std /= in Hy;auto.
+       + rewrite std_sta_update_multiple_lookup_same_i /= in Hx;auto.
+         rewrite std_sta_update_multiple_lookup_same_i /= in Hy;auto.
          apply Hstd_related with i; auto.
    Qed.
 
@@ -374,8 +387,8 @@ Section std_updates.
        rewrite lookup_insert_ne; auto.
      - rewrite std_sta_update_multiple_lookup_same_i; auto.
        destruct (decide ( a' =  l)).
-       + rewrite /std_update /std /= e. do 2 rewrite lookup_insert. done.
-       + rewrite /std_update /std /=. rewrite lookup_insert_ne;auto. rewrite lookup_insert_ne; auto.
+       + rewrite /std_update /= e. do 2 rewrite lookup_insert. done.
+       + rewrite /std_update /=. rewrite lookup_insert_ne;auto. rewrite lookup_insert_ne; auto.
          rewrite std_sta_update_multiple_lookup_same_i; auto.
    Qed.
 
@@ -384,7 +397,7 @@ Section std_updates.
      Forall (λ a : Addr,
                    (a ∉ dom (std W))) (finz.seq_between a b) →
      Forall (λ a : Addr,
-                   (a ∉ dom (<[ a' := i]> W.1))) (finz.seq_between a b).
+                   (a ∉ dom (<[ a' := i]> (std W)))) (finz.seq_between a b).
    Proof.
      intros Hlt.
      do 2 (rewrite list.Forall_forall). intros Hforall.
@@ -420,7 +433,9 @@ Section std_updates.
      std_update_multiple (std_update_multiple W l ρ1) l ρ2 = std_update_multiple W l ρ2.
    Proof.
      induction l;auto.
-     simpl. destruct W as [Wstd Wloc]. rewrite /std_update /=. rewrite !std_update_multiple_loc /=. f_equiv.
+     simpl. destruct W as [Wstd Wloc]. rewrite /std_update /=.
+     rewrite !std_update_multiple_cus /=; f_equiv.
+     all: rewrite !std_update_multiple_frm /=; f_equiv.
      apply map_eq'. intros k v.
      destruct (decide (a = k)).
      + subst. rewrite !lookup_insert. auto.
@@ -438,7 +453,7 @@ Section std_updates.
      induction l; auto; simpl.
      apply not_elem_of_cons in Hne as [Hne Hnin].
      rewrite IHl;auto.
-     rewrite /std_update /loc /std /=. rewrite insert_commute;auto.
+     rewrite /std_update /=. rewrite insert_commute;auto.
    Qed.
 
    Lemma related_sts_pub_world_revoked_permanent W a :
@@ -447,7 +462,7 @@ Section std_updates.
   Proof.
     intros Ha.
     rewrite /related_sts_pub_world /=.
-    split;[|apply related_sts_pub_refl].
+    split;[split|];[|apply related_sts_pub_refl|apply related_tframe_pub_refl].
     rewrite /related_sts_pub. split.
     - rewrite dom_insert_L. set_solver.
     - intros i x y Hx Hy.
@@ -474,7 +489,7 @@ Section std_updates.
        destruct (decide (a ∈ l)).
        { rewrite (_: <s[a:=Permanent]s>(std_update_multiple W l Permanent) = std_update_multiple W l Permanent) /=.
          by apply related_sts_pub_refl_world.
-         rewrite /std_update insert_id /=. by destruct (std_update_multiple W l Permanent).
+         rewrite /std_update insert_id /=. by destruct (std_update_multiple W l Permanent) as [ [] ].
          by apply std_sta_update_multiple_lookup_in_i. }
        destruct W as [Hstd Hloc].
        apply related_sts_pub_world_revoked_permanent in Ha_std.
@@ -488,7 +503,7 @@ Section std_updates.
    Proof.
      intros Ha.
      rewrite /related_sts_pub_world /=.
-     split;[|apply related_sts_pub_refl].
+    split;[split|];[|apply related_sts_pub_refl|apply related_tframe_pub_refl].
      rewrite /related_sts_pub. split.
      - rewrite dom_insert_L. set_solver.
      - intros i x y Hx Hy.
@@ -515,7 +530,7 @@ Section std_updates.
        destruct (decide (a ∈ l)).
        { rewrite (_: <s[a:=Temporary]s>(std_update_multiple W l Temporary) = std_update_multiple W l Temporary) /=.
          by apply related_sts_pub_refl_world.
-         rewrite /std_update insert_id /=. by destruct (std_update_multiple W l Temporary).
+         rewrite /std_update insert_id /=. by destruct (std_update_multiple W l Temporary) as [ [] ].
          by apply std_sta_update_multiple_lookup_in_i. }
        destruct W as [Hstd Hloc].
        apply related_sts_pub_world_revoked_temporary in Ha_std.
@@ -532,7 +547,7 @@ Section std_updates.
      destruct (decide (a = a')) as [|Hna]; simplify_eq; first (left; set_solver).
      destruct (decide (a ∈ l)) as [|Hnl]; first (left; set_solver).
      right.
-     rewrite /= /std dom_insert_L elem_of_union in Ha.
+     rewrite /= dom_insert_L elem_of_union in Ha.
      destruct Ha as [Ha|Ha] ; first ( rewrite elem_of_singleton in Ha ; set_solver ).
      apply IHl in Ha. destruct Ha; done.
    Qed.
