theories/region_invariants_allocation.v
@@ -8,13 +8,14 @@ Section region_alloc.
   Context {Σ:gFunctors}
     {ceriseg:ceriseG Σ}
     {Cname : CmptNameG}
-    {stsg : STSG Addr region_type Σ}
+    {stsg : STSG Addr region_type Σ} {tframeg : TFRAMEG Σ}
     {heapg : heapGS Σ}
     `{MP: MachineParameters}.
 
   Notation STS := (leibnizO (STS_states * STS_rels)).
   Notation STS_STD := (leibnizO (STS_std_states Addr region_type)).
-  Notation WORLD := (prodO STS_STD STS).
+  Notation TFRAME := (leibnizO nat).
+  Notation WORLD := ( prodO (prodO STS_STD STS) TFRAME) .
   Implicit Types W : WORLD.
   Implicit Types C : CmptName.
 
@@ -57,7 +58,7 @@ Section region_alloc.
     iModIntro. rewrite bi.sep_exist_r. iExists _.
     iFrame "HR ∗ #".
     iExists (<[a:=_]> Mρ);iSplitR;[|iSplitR].
-    - iPureIntro. rewrite /std /std_update in HMW |- *.
+    - iPureIntro. rewrite /std_update in HMW |- *.
       repeat rewrite dom_insert_L; rewrite HMW; auto.
     - iPureIntro. repeat rewrite dom_insert_L. rewrite HMρ. auto.
     - iApply big_sepM_insert; auto.
@@ -116,7 +117,7 @@ Section region_alloc.
     iModIntro. rewrite bi.sep_exist_r. iExists _.
     iFrame "HR ∗ #".
     iExists (<[a:=_]> Mρ);iSplitR;[|iSplitR].
-    - iPureIntro. rewrite /std /std_update in HMW |- *.
+    - iPureIntro. rewrite /std_update in HMW |- *.
       repeat rewrite dom_insert_L; rewrite HMW; auto.
     - iPureIntro. repeat rewrite dom_insert_L. rewrite HMρ. auto.
     - iApply big_sepM_insert; auto.
@@ -198,7 +199,7 @@ Section region_alloc.
     iModIntro. rewrite bi.sep_exist_r. iExists _.
     iFrame "HR ∗ #".
     iExists (<[a:=_]> Mρ);iSplitR;[|iSplitR].
-    - iPureIntro. rewrite /std /std_update in HMW |- *.
+    - iPureIntro. rewrite /std_update in HMW |- *.
       repeat rewrite dom_insert_L; rewrite HMW; auto.
     - iPureIntro. repeat rewrite dom_insert_L. rewrite HMρ. auto.
     - iApply big_sepM_insert; auto.
@@ -255,7 +256,7 @@ Section region_alloc.
     iModIntro. rewrite bi.sep_exist_r. iExists _.
     iFrame "HR ∗ #".
     iExists (<[a:=_]> Mρ);iSplitR;[|iSplitR].
-    - iPureIntro. rewrite /std /std_update in HMW |- *.
+    - iPureIntro. rewrite /std_update in HMW |- *.
       repeat rewrite dom_insert_L; rewrite HMW; auto.
     - iPureIntro. repeat rewrite dom_insert_L. rewrite HMρ. auto.
     - iApply big_sepM_insert; auto.
@@ -295,23 +296,22 @@ Section region_alloc.
         assert (<s[a:=Revoked]s>(std_update_multiple W l1 Revoked)
                 = std_update_multiple W l1 Revoked) as ->.
         { rewrite /std_update.
-          destruct (std_update_multiple W l1 Revoked) eqn:Heq.
+          destruct (std_update_multiple W l1 Revoked) as [ [] ] eqn:Heq.
+          f_equiv; last done.
           f_equiv; last done.
           simpl. rewrite insert_id//.
-          assert (o = (std_update_multiple W l1 Revoked).1) as ->;[rewrite Heq//|].
+          assert (o = std (std_update_multiple W l1 Revoked)) as ->;[rewrite Heq//|].
           apply std_sta_update_multiple_lookup_in_i;auto.
         }
         destruct (std_update_multiple W l1 Revoked) as [Wstd_sta Wloc] eqn:Heq.
         destruct l1; first by rewrite lookup_nil in Hk.
         by iFrame "#∗".
       + iMod (extend_region_revoked _ _ _ a with "Hsts Hr") as "(Hr & Hrel & Hsts)"; auto.
-        { rewrite /std in H0.
-          destruct l1.
+        { destruct l1.
           { rewrite not_elem_of_dom //. }
           rewrite -std_update_multiple_not_in_sta; auto.
           rewrite not_elem_of_dom //.
         }
-        rewrite /std in H0.
         by iFrame "#∗".
   Qed.
 
